docs/dafny/ExamplesExternUniform.dfy
@@ -8,6 +8,7 @@
 include "../../src/Dafny-VMC.dfy"
 
 module RandomExamples {
+  import Rationals
   import DafnyVMC
 
   method Main()
@@ -69,7 +70,7 @@ module RandomExamples {
 
     t := 0;
     for i := 0 to n {
-      var b := r.BernoulliRational(1, 5);
+      var b := r.BernoulliRational(Rationals.Rational(1, 5));
       if b {
         t := t + 1;
       }
@@ -79,7 +80,7 @@ module RandomExamples {
 
     t := 0;
     for i := 0 to n {
-      var b := r.BernoulliRational(0, 5);
+      var b := r.BernoulliRational(Rationals.Rational(0, 5));
       if b {
         t := t + 1;
       }
@@ -89,7 +90,7 @@ module RandomExamples {
 
     t := 0;
     for i := 0 to n {
-      var b := r.BernoulliRational(5, 5);
+      var b := r.BernoulliRational(Rationals.Rational(5, 5));
       if b {
         t := t + 1;
       }
@@ -110,7 +111,7 @@ module RandomExamples {
 
     t := 0;
     for i := 0 to n {
-      var u := r.BernoulliExpNeg(2.30258509299); // about -ln(0.1)
+      var u := r.BernoulliExpNeg(Rationals.Rational(12381, 5377)); // about -ln(0.1)
       if u {
         t := t + 1;
       }
@@ -121,7 +122,7 @@ module RandomExamples {
     var count1 := 0;
     var countneg1 := 0;
     for i := 0 to n {
-      var u := r.DiscreteLaplace(5, 7); // DiscreteLaplace(7/5)
+      var u := r.DiscreteLaplace(Rationals.Rational(7, 5));
       match u {
         case -1 => countneg1 := countneg1 + 1;
         case 0 => count0 := count0 + 1;
@@ -138,7 +139,7 @@ module RandomExamples {
     count1 := 0;
     countneg1 := 0;
     for i := 0 to n {
-      var u := r.DiscreteGaussian(1.4);
+      var u := r.DiscreteGaussian(Rationals.Rational(7, 5));
       match u {
         case -1 => countneg1 := countneg1 + 1;
         case 0 => count0 := count0 + 1;
